Math/TypeTheory/LambdaV2/Basic.lean
@@ -1,0 +1,173 @@
+import Math.Data.Multiset.Basic
+
+inductive LamType where
+| Void
+| Unit
+| Func (arg ret: LamType)
+deriving DecidableEq
+
+inductive LamTerm where
+| ConstUnit
+| Panic (body: LamTerm) (ty: LamType)
+| Lambda (arg_name: Nat) (arg_ty: LamType) (body: LamTerm)
+| App (func arg: LamTerm)
+| Var (name: Nat)
+
+structure Context: Type where
+  data: Multiset (Nat × LamType)
+  nodup_keys: data.Pairwise <| fun x y => x.1 ≠ y.1
+
+instance : Membership Nat Context where
+  mem ctx name := ∃v, ⟨name, v⟩ ∈ ctx.data
+
+instance (x: Nat) (ctx: Context) : Decidable (x ∈ ctx) :=
+  decidable_of_iff (∃y ∈ ctx.data, x = y.1) <| by
+    apply Iff.intro
+    intro ⟨⟨k, v⟩, mem, eq⟩
+    exists v
+    subst x
+    assumption
+    intro ⟨v, mem⟩
+    exists ⟨x, v⟩
+
+-- inserts key into ctx iff it doesn't already exist in ctx
+def Context.insert (key: Nat) (ty: LamType) (ctx: Context) : Context where
+  data :=
+    if key ∈ ctx then
+      ctx.data
+    else
+      ⟨key, ty⟩ ::ₘ ctx.data
+  nodup_keys := by
+    split <;> rename_i h
+    exact ctx.nodup_keys
+    apply ctx.nodup_keys.cons
+    intro ⟨k, v⟩ mem eq
+    apply h
+    dsimp at eq
+    subst k
+    exists v
+
+instance : EmptyCollection Context where
+  emptyCollection := { data := ∅, nodup_keys := Multiset.Pairwise.nil }
+
+instance : Insert (Nat × LamType) Context where
+  insert x := Context.insert x.1 x.2
+
+instance : Singleton (Nat × LamType) Context where
+  singleton := (insert · ∅)
+
+instance : GetElem Context Nat LamType (fun ctx name => name ∈ ctx) where
+  getElem ctx name prf := by
+    apply Quotient.hrecOn ctx.data (motive := fun list => (∃v, Multiset.mem  ⟨name, v⟩ list) -> Multiset.Pairwise (fun x y => x.1 ≠ y.1) list -> LamType)
+    case f =>
+      intro list mem _
+      apply Option.getD _ LamType.Void
+      apply Option.map _
+      exact list.find? fun ⟨k, v⟩ => k = name
+      exact Prod.snd
+    case c =>
+      dsimp
+      intro a b eq
+      apply Function.hfunext
+      · show (∃v, (name, v) ∈ Multiset.mk _) = (∃v, (name, v) ∈ Multiset.mk _)
+        congr
+        funext
+        congr 1
+        apply Quotient.sound
+        assumption
+      intro h₀ h₁ heq₁
+      apply Function.hfunext
+      · congr 1
+        apply Quotient.sound
+        assumption
+      intro h₂ h₃ heq₂
+      apply heq_of_eq
+      clear h₀ h₁ heq₁
+      · induction eq with
+        | nil => rfl
+        | cons _ _ ih =>
+          unfold List.find?
+          split
+          rfl
+          apply ih
+          apply proof_irrel_heq
+          cases h₂
+          assumption
+          cases h₃
+          assumption
+        | trans _ _ ih₀ ih₁ =>
+          rename_i x₀ x₁ x₂ x₁₂ x₂₃
+          have : Multiset.Pairwise (fun x y => x.1 ≠ y.1) (Quotient.mk _ x₁) := by
+            rw [Quotient.sound x₂₃]
+            assumption
+          rw [ih₀, ih₁]
+          any_goals assumption
+          any_goals apply proof_irrel_heq
+        | swap =>
+          unfold List.find? List.find?
+          rename_i x y _
+          cases hx:decide (x.fst = name) <;> cases hy:decide (y.fst = name) <;> dsimp
+          exfalso
+          cases h₂
+          rename_i h
+          apply h
+          apply List.Mem.head
+          rw [of_decide_eq_true hx, of_decide_eq_true hy]
+    case a => exact prf
+    case a => exact ctx.nodup_keys
+
+def Context.mem_insert_head (key: Nat) (ty: LamType) (ctx: Context) :
+  key ∈ ctx.insert key ty := by
+  unfold insert
+  split
+  rename_i h
+  show ∃_, _
+  assumption
+  exists ty
+  apply Multiset.mem_head
+
+def Context.mem_insert_tail (k key: Nat) (ty: LamType) (ctx: Context) :
+  k ∈ ctx ->
+  k ∈ ctx.insert key ty := by
+  intro h
+  unfold insert
+  split
+  rename_i h
+  show ∃_, _
+  assumption
+  obtain ⟨v, mem⟩ := h
+  exists v
+  apply Multiset.mem_tail
+  assumption
+
+macro_rules
+| `(tactic|get_elem_tactic_trivial) => `(tactic|apply Context.mem_insert_head)
+macro_rules
+| `(tactic|get_elem_tactic_trivial) => `(tactic|apply Context.mem_insert_tail; get_elem_tactic)
+
+def Context.insert_get_elem_head (ctx: Context) (key: Nat) (ty: LamType) (h: key ∉ ctx) : (ctx.insert key ty)[key] = ty := by
+  unfold insert
+  cases ctx with | mk ctx nodup =>
+  cases ctx with | mk ctx =>
+  split <;> show Option.getD _ LamType.Void = _
+  contradiction
+  unfold List.find?
+  dsimp
+  rw [decide_eq_true_iff.mpr rfl]
+  rfl
+
+def Context.insert_get_elem_tail (ctx: Context) (key k: Nat) (ty: LamType) (h: k ∈ ctx) : (ctx.insert key ty)[k] = ctx[k] := by
+  unfold insert
+  cases ctx with | mk ctx nodup =>
+  cases ctx with | mk ctx =>
+  split <;> show Option.getD _ LamType.Void = _
+  rfl
+  have k_ne_key : k ≠ key := by
+    intro eq
+    cases eq; contradiction
+  unfold List.find?
+  dsimp
+  rw [decide_eq_false_iff_not.mpr k_ne_key.symm]
+  rfl
+
+infix:65 "::*" => Context.push
